theories/sta_inv.v
@@ -1,0 +1,119 @@
+From mathcomp Require Import ssreflect ssrbool eqtype ssrnat seq.
+From Coq Require Import ssrfun Classical Utf8.
+Require Export AutosubstSsr ARS sta_subst.
+
+Set Implicit Arguments.
+Unset Strict Implicit.
+Unset Printing Implicit Defensive.
+
+Lemma sta_pi0_inv Γ A B C s t :
+  Γ ⊢ Pi0 A B s t : C ->
+  exists2 r, Γ ⊢ A : @s & (A :: Γ) ⊢ B : @r.
+Proof with eauto.
+  move e:(Pi0 A B s t)=>m ty.
+  elim: ty A B s t e=>//{Γ C m}.
+  move=>Γ A B s r t tyA ihA tyB ihB A0 B0 s0 t0
+    [e1 e2 e3 e4]; subst.
+  exists r...
+Qed.
+
+Lemma sta_pi1_inv Γ A B C s t :
+  Γ ⊢ Pi1 A B s t : C ->
+  exists2 r, Γ ⊢ A : @s & (A :: Γ) ⊢ B : @r.
+Proof with eauto.
+  move e:(Pi1 A B s t)=>m ty.
+  elim: ty A B s t e=>//{Γ C m}.
+  move=>Γ A B s r t tyA ihA tyB ihB A0 B0 s0 t0
+    [e1 e2 e3 e4]; subst.
+  exists r...
+Qed.
+
+Lemma sta_lam0_invX Γ A1 A2 B C m s1 s2 t1 t2 r :
+  Γ ⊢ Lam0 A1 m s1 t1 : C ->
+  C === Pi0 A2 B s2 t2 ->
+  (A2 :: Γ) ⊢ B : @r ->
+  (A2 :: Γ) ⊢ m : B.
+Proof with eauto.
+  move e:(Lam0 A1 m s1 t1)=>n tyL.
+  elim: tyL A1 A2 B m s1 s2 t1 t2 r e=>//{Γ C n}.
+  { move=>Γ A B m s t tyP ihP tym ihm A1 A2 B0 m0
+      s1 s2 t1 t2 r0 [e1 e2 e3 e4]/pi0_inj[eq1[eq2[e5 e6]]] tyB0; subst.
+    have[r tyA tyB]:=sta_pi0_inv tyP.
+    apply: sta_conv...
+    apply: sta_ctx_conv.
+    apply: (conv_sym eq1).
+    exact: tyA.
+    exact: tym. }
+  { move=>Γ A B m s eq1 tym ihm tyB ihB A1 A2 B0 m0
+      s1 s2 t1 t2 r e eq2 tyB0; subst.
+    apply: ihm...
+    apply: conv_trans... }
+Qed.
+
+Lemma sta_lam1_invX Γ A1 A2 B C m s1 s2 t1 t2 r :
+  Γ ⊢ Lam1 A1 m s1 t1 : C ->
+  C === Pi1 A2 B s2 t2 ->
+  (A2 :: Γ) ⊢ B : @r ->
+  (A2 :: Γ) ⊢ m : B.
+Proof with eauto.
+  move e:(Lam1 A1 m s1 t1)=>n tyL.
+  elim: tyL A1 A2 B m s1 s2 t1 t2 r e=>//{Γ C n}.
+  { move=>Γ A B m s t tyP ihP tym ihm A1 A2 B0 m0
+      s1 s2 t1 t2 r0 [e1 e2 e3 e4]/pi1_inj[eq1[eq2[e5 e6]]] tyB0; subst.
+    have[r tyA tyB]:=sta_pi1_inv tyP.
+    apply: sta_conv...
+    apply: sta_ctx_conv.
+    apply: (conv_sym eq1).
+    exact: tyA.
+    exact: tym. }
+  { move=>Γ A B m s eq1 tym ihm tyB ihB A1 A2 B0 m0
+      s1 s2 t1 t2 r e eq2 tyB0; subst.
+    apply: ihm...
+    apply: conv_trans... }
+Qed.
+
+Lemma sta_lam0_inv Γ m A1 A2 B s1 s2 t1 t2 x :
+  Γ ⊢ Pi0 A1 B s1 t1 : @x ->
+  Γ ⊢ Lam0 A2 m s2 t2 : Pi0 A1 B s1 t1 ->
+  (A1 :: Γ) ⊢ m : B.
+Proof with eauto.
+  move=>/sta_pi0_inv[r tyA1 tyB] tyL.
+  apply: sta_lam0_invX...
+Qed.
+
+Lemma sta_lam1_inv Γ m A1 A2 B s1 s2 t1 t2 x :
+  Γ ⊢ Pi1 A1 B s1 t1 : @x ->
+  Γ ⊢ Lam1 A2 m s2 t2 : Pi1 A1 B s1 t1 ->
+  (A1 :: Γ) ⊢ m : B.
+Proof with eauto.
+  move=>/sta_pi1_inv[r tyA1 tyB] tyL.
+  apply: sta_lam1_invX...
+Qed.
+
+Lemma sta_lam0_pi1_false Γ A1 A2 B C m s1 s2 t1 t2 :
+  Γ ⊢ Lam0 A1 m s1 t1 : C -> C === Pi1 A2 B s2 t2 -> False.
+Proof with eauto.
+  move e:(Lam0 A1 m s1 t1)=>n tyL.
+  elim: tyL A1 A2 B m s1 s2 t1 t2 e=>//{Γ C n}.
+  { move=>Γ A B m s t tyP ihP tym ihm A1 A2 B0 m0
+      s1 s2 t1 t2 [e1 e2 e3 e4] eq; subst.
+    solve_conv. }
+  { move=>Γ A B m s eq1 tym ihm tyB ihB A1 A2 B0 m0
+      s1 s2 t1 t2 e eq2; subst.
+    apply: ihm...
+    apply: conv_trans... }
+Qed.
+
+Lemma sta_lam1_pi0_false Γ A1 A2 B C m s1 s2 t1 t2 :
+  Γ ⊢ Lam1 A1 m s1 t1 : C -> C === Pi0 A2 B s2 t2 -> False.
+Proof with eauto.
+  move e:(Lam1 A1 m s1 t1)=>n tyL.
+  elim: tyL A1 A2 B m s1 s2 t1 t2 e=>//{Γ C n}.
+  { move=>Γ A B m s t tyP ihP tym ihm A1 A2 B0 m0
+      s1 s2 t1 t2 [e1 e2 e3 e4] eq; subst.
+    solve_conv. }
+  { move=>Γ A B m s eq1 tym ihm tyB ihB A1 A2 B0 m0
+      s1 s2 t1 t2 e eq2; subst.
+    apply: ihm...
+    apply: conv_trans... }
+Qed.
