theories/sta_valid.v
@@ -1,0 +1,20 @@
+From mathcomp Require Import ssreflect ssrbool eqtype ssrnat seq.
+From Coq Require Import ssrfun Classical Utf8.
+Require Export AutosubstSsr ARS sta_inv.
+
+Set Implicit Arguments.
+Unset Strict Implicit.
+Unset Printing Implicit Defensive.
+
+Theorem sta_valid Γ m A : sta_wf Γ -> Γ ⊢ m : A -> exists s, Γ ⊢ A : @s.
+Proof with eauto using sta_type.
+  move=>wf ty. elim: ty wf=>{Γ m A}...
+  { move=>Γ x A hs wf.
+    apply: sta_wf_ok... }
+  { move=>Γ A B m n s t tym ihm tyn ihn wf.
+    have[_/sta_pi0_inv[r tyA tyB]]:=ihm wf.
+    exists r. have//:=sta_subst tyB tyn. }
+  { move=>Γ A B m n s t tym ihm tyn ihn wf.
+    have[_/sta_pi1_inv[r tyA tyB]]:=ihm wf.
+    exists r. have//:=sta_subst tyB tyn. }
+Qed.
